Tweak the QD output

src/tls/QD.TLS_protocolVersion.fst
@@ -23,7 +23,7 @@ inline_for_extraction let synth_protocolVersion' (x:LP.maybe_enum_key protocolVe
   | LP.Known k -> k
   | LP.Unknown y ->
     [@inline_let] let v : UInt16.t = y in
-    [@inline_let] let _ = norm_spec LP.norm_steps (LP.list_mem v (LP.list_map snd protocolVersion_enum)) in
+    [@inline_let] let _ = LP.norm_spec (LP.list_mem v (LP.list_map snd protocolVersion_enum)) in
     Unknown_protocolVersion v
 
 let lemma_synth_protocolVersion'_inj () : Lemma
@@ -34,11 +34,11 @@ inline_for_extraction let synth_protocolVersion'_inv (x:protocolVersion') : Tot 
   match x with
   | Unknown_protocolVersion y ->
     [@inline_let] let v : UInt16.t = y in
-    [@inline_let] let _ = norm_spec LP.norm_steps (LP.list_mem v (LP.list_map snd protocolVersion_enum)) in
+    [@inline_let] let _ = LP.norm_spec (LP.list_mem v (LP.list_map snd protocolVersion_enum)) in
     LP.Unknown v
   | x ->
     [@inline_let] let x1 : protocolVersion = x in
-    [@inline_let] let _ = norm_spec LP.norm_steps (LP.list_mem x1 (LP.list_map fst protocolVersion_enum)) in
+    [@inline_let] let _ = LP.norm_spec (LP.list_mem x1 (LP.list_map fst protocolVersion_enum)) in
     LP.Known (x1 <: LP.enum_key protocolVersion_enum)
 
 let lemma_synth_protocolVersion'_inv () : Lemma
@@ -50,11 +50,11 @@ let parse_maybe_protocolVersion_key : LP.parser _ (LP.maybe_enum_key protocolVer
 let serialize_maybe_protocolVersion_key : LP.serializer parse_maybe_protocolVersion_key =
   LP.serialize_maybe_enum_key LP.parse_u16 LP.serialize_u16 protocolVersion_enum
 
-let parse_protocolVersion' : LP.parser _ protocolVersion' =
+let spec_parse_protocolVersion' : LP.parser _ protocolVersion' =
   lemma_synth_protocolVersion'_inj ();
   parse_maybe_protocolVersion_key `LP.parse_synth` synth_protocolVersion'
 
-let serialize_protocolVersion' : LP.serializer parse_protocolVersion' =
+let serialize_protocolVersion' : LP.serializer spec_parse_protocolVersion' =
   lemma_synth_protocolVersion'_inj ();
   lemma_synth_protocolVersion'_inv ();
   LP.serialize_synth _ synth_protocolVersion' serialize_maybe_protocolVersion_key synth_protocolVersion'_inv ()
@@ -62,7 +62,7 @@ let serialize_protocolVersion' : LP.serializer parse_protocolVersion' =
 inline_for_extraction let parse32_maybe_protocolVersion_key : LP.parser32 parse_maybe_protocolVersion_key =
   FStar.Tactics.synth_by_tactic (LP.parse32_maybe_enum_key_tac LP.parse32_u16 protocolVersion_enum parse_maybe_protocolVersion_key ())
 
-inline_for_extraction let parse32_protocolVersion' : LP.parser32 parse_protocolVersion' =
+inline_for_extraction let parse32_protocolVersion' : LP.parser32 spec_parse_protocolVersion' =
   lemma_synth_protocolVersion'_inj ();
   LP.parse32_synth _ synth_protocolVersion' (fun x->synth_protocolVersion' x) parse32_maybe_protocolVersion_key ()
 
@@ -76,17 +76,40 @@ inline_for_extraction let serialize32_protocolVersion' : LP.serializer32 seriali
   lemma_synth_protocolVersion'_inv ();
   LP.serialize32_synth _ synth_protocolVersion' _ serialize32_maybe_protocolVersion_key synth_protocolVersion'_inv (fun x->synth_protocolVersion'_inv x) ()
 
-let protocolVersion_bytes x = serialize32_protocolVersion' x <: LP.bytes32
+let protocolVersion_bytes x =
+  LowParseWrappers.wrap_serializer32_constant_length serialize32_protocolVersion' 2 () x
+
+open FStar.Error
+
+inline_for_extraction
+let parse_protocolVersion_error_msg : string =
+  FStar.Error.perror __SOURCE_FILE__ __LINE__ ""
 
 let parse_protocolVersion' x =
-  LP.parse32_total parse32_protocolVersion' v;
-  match parse32_protocolVersion' x with
-  | Some (v, _) -> Correct v
-  | None -> Error (AD_decode_error, perror __SOURCE_FILE__ __LINE__ "")
+  LowParseWrappers.wrap_parser32_constant_length serialize32_protocolVersion' 2 () parse32_protocolVersion' parse_protocolVersion_error_msg x
+
+(* TODO: use LP.parse32/serialize32_enum_key instead. The problem here
+is that we want to prove that the same serializer will work for both
+protocolVersion' and protocolVersion, for which the proof will take
+10 seconds instead of 1. *)
 
 let parse_protocolVersion x =
-  LP.parse32_total parse32_protocolVersion' v;
-  match parse32_protocolVersion' x with
-  | Some (v, _) -> if v = Unknown_protocolVersion then Error (AD_decode_error, perror __SOURCE_FILE__ __LINE__ "") else Correct v
-  | None -> Error (AD_decode_error, perror __SOURCE_FILE__ __LINE__ "")
+  let k : result protocolVersion' = parse_protocolVersion' x in
+  match k with
+  | Correct c ->
+    if Unknown_protocolVersion? c
+    then
+      Error (AD_decode_error, perror __SOURCE_FILE__ __LINE__ "")
+    else begin
+      Correct c
+    end
+  | _ ->
+    assert (Error? k); // FIXME: WHY WHY WHY is this assert necessary? If not there, then proof fails.
+    let (Error e) = k in
+    Error e
 
+let inverse_protocolVersion' x =
+  LowParseWrappers.lemma_inverse_serializer32_parser32_constant_length serialize32_protocolVersion' 2 () parse32_protocolVersion' parse_protocolVersion_error_msg x
+
+let pinverse_protocolVersion' x =
+  LowParseWrappers.lemma_pinverse_serializer32_parser32_constant_length serialize32_protocolVersion' 2 () parse32_protocolVersion' parse_protocolVersion_error_msg x
