src/tls/QD.TLS_protocolVersion.fsti
@@ -2,6 +2,7 @@ module QD.TLS_protocolVersion
 
 open FStar.Bytes
 open TLSError
+open Parse
 
 type protocolVersion' =
   | SSL_3p0
@@ -14,5 +15,13 @@ type protocolVersion' =
 type protocolVersion = v:protocolVersion'{~(Unknown_protocolVersion? v)}
 
 inline_for_extraction val protocolVersion_bytes: protocolVersion' -> Tot (lbytes 2)
-inline_for_extraction val parse_protocolVersion': bytes -> result protocolVersion'
-inline_for_extraction val parse_protocolVersion: bytes -> result protocolVersion
+inline_for_extraction val parse_protocolVersion': lbytes 2 -> result protocolVersion'
+inline_for_extraction val parse_protocolVersion: lbytes 2 -> result protocolVersion
+
+val inverse_protocolVersion' (x:_) : Lemma
+  (requires True)
+  (ensures lemma_inverse_g_f protocolVersion_bytes parse_protocolVersion' x)
+
+val pinverse_protocolVersion' (x:_) : Lemma
+  (requires True)
+  (ensures lemma_pinverse_f_g equal protocolVersion_bytes parse_protocolVersion' x)
